Flesh out stack operations, fix lifting use

SimAsm/SimAsm_StateStack.thy
@@ -39,14 +39,15 @@ setup_lifting type_definition_frame_ext
 copy_bnf ('a,'b,'c) frame_ext
 print_quot_maps
   
-type_synonym ('var,'val,'a) stack = "('var, 'val,'a) frame_scheme list" 
+type_synonym ('var,'val,'a) stack = "('var, 'val,'a option) frame_scheme list"
 
-definition emptyFrame :: "'var set \<Rightarrow> ('var,'val) frame" where
+definition emptyFrame :: "'var set \<Rightarrow> ('var,'val,'a option) frame_scheme" where
   "emptyFrame cap \<equiv> \<lparr> frame_st = (\<lambda>v. None),
-                  frame_cap = cap \<rparr>"            (* is cap set as parameter *)
+                      frame_cap = cap,
+                      \<dots> = None \<rparr>"            (* is cap set as parameter *)
 
 definition Is_tstack :: "('var,'val,'a) stack \<Rightarrow> bool" where 
-  "Is_tstack t \<equiv> t \<noteq> [] \<and> frame_cap (last t) = UNIV \<and> (\<forall>v. frame_st (last t) v \<noteq> None)"
+  "Is_tstack t \<equiv> t \<noteq> [] \<and> frame_cap (last t) = UNIV \<and> (\<forall>v. frame_st (last t) v \<noteq> None) \<and> more (last t) \<noteq> None"
 
 lemma Is_tstack_ConsI [intro]: "Is_tstack xs \<Longrightarrow> Is_tstack (x#xs)" 
 unfolding Is_tstack_def  
@@ -88,17 +89,20 @@ typedef ('var,'val,'a) tstack = "{t :: ('var,'val,'a) stack. Is_tstack t}"
 unfolding Is_tstack_def
 proof (standard, clarify, intro conjI allI)
   fix x a
-  let ?f = "\<lparr>frame_st = \<lambda>_. Some x, frame_cap = UNIV, \<dots> = a\<rparr> :: ('var,'val,'a) frame_scheme" 
+  let ?f = "\<lparr>frame_st = \<lambda>_. Some x, frame_cap = UNIV, \<dots> = Some a\<rparr> :: ('var,'val,'a option) frame_scheme"
   have last: "last [?f] = ?f" using last_ConsL by fast
   show "[?f] \<noteq> []" by fast
   show "frame_st (last [?f]) v \<noteq> None" for v
     unfolding last select_convs(1) by simp
   show "frame_cap (last [?f]) = UNIV"
     unfolding last select_convs(2) by simp
+  show "more (last [?f]) \<noteq> None"
+    unfolding last by simp
 qed
 
-setup_lifting type_definition_tstack    
+setup_lifting type_definition_tstack
 
+(*
 (* declare Abs_tstack_inverse[intro] *)
 find_theorems Abs_tstack
 
@@ -115,19 +119,20 @@ lemma Rep_tstackI [intro!]:
     "x \<in> frame_cap (last (Rep_tstack s))" 
     "frame_st (last (Rep_tstack s)) v \<noteq> None" 
 by (induct s) (auto simp add: Abs_tstack_inverse)
+*)
 
-lemma Is_tstack_induct [case_names Base Frame Is_tstack]:
-assumes "\<And>x. Is_tstack [x] \<Longrightarrow> P [x]"
-assumes "\<And>x xs. P xs \<Longrightarrow> Is_tstack xs \<Longrightarrow> P (x#xs)"
-assumes "Is_tstack s"
-shows "P s"
-using assms
+lemma Is_tstack_induct [consumes 1, case_names Base Frame]:
+  assumes "Is_tstack s"
+  assumes "\<And>x. frame_cap x = UNIV \<Longrightarrow> (\<forall>v. frame_st x v \<noteq> None) \<Longrightarrow> more x \<noteq> None \<Longrightarrow> P [x]"
+  assumes "\<And>x xs. P xs \<Longrightarrow> Is_tstack xs \<Longrightarrow> P (x#xs)"
+  shows "P s"
+  using assms
 proof (induct s)
   case (Cons a s)
-  thus ?case 
-  by (cases s) (auto intro: assms)
+  thus ?case by (cases s) (auto intro: assms simp: Is_tstack_def)
 qed auto
 
+(*
 lemma tstack_induct [case_names Base Frame]: 
 assumes "\<And>x. Is_tstack [x] \<Longrightarrow> P (Abs_tstack [x])"
 assumes "\<And>x xs. P (Abs_tstack xs) \<Longrightarrow> Is_tstack xs \<Longrightarrow> P (Abs_tstack (x#xs))"
@@ -140,12 +145,12 @@ proof (induct s)
     case (Is_tstack)
     thus ?case using Abs_tstack by auto
   qed auto
-qed 
+qed *)
 
 lemma Is_tstack_snoc: "Is_tstack xs \<Longrightarrow> Is_tstack (butlast xs @ [last xs])"
 unfolding Is_tstack_def by simp
 
-lemma Is_tstack_snoc_moreupd: "Is_tstack xs \<Longrightarrow> Is_tstack (butlast xs @ [last xs\<lparr> more := any \<rparr>])"
+lemma Is_tstack_snoc_moreupd: "Is_tstack xs \<Longrightarrow> Is_tstack (butlast xs @ [last xs\<lparr> more := Some any \<rparr>])"
 unfolding Is_tstack_def by simp
 
 
@@ -158,105 +163,313 @@ fun update :: "('var,'val,'a) stack \<Rightarrow> 'var \<Rightarrow> 'val \<Righ
   "update [] _ _ = undefined" |
   "update (f#fs) v x = (if (v \<in> frame_cap f) then (f\<lparr>frame_st := (frame_st f)(v \<mapsto> x)\<rparr>)#fs else f#update fs v x)"
 
-lift_definition tlookup :: "('var,'val,'a) tstack \<Rightarrow> 'var \<Rightarrow> 'val" 
-  is "\<lambda>fs v. lookup (Rep_tstack fs) v".
-  
-lift_definition tupdate :: "('var,'val,'a) tstack \<Rightarrow> 'var \<Rightarrow> 'val \<Rightarrow> ('var,'val,'a) tstack"
-  is "\<lambda>fs v x. Abs_tstack (update (Rep_tstack fs) v x)".
-
-lift_definition taux :: "('var,'val,'a) tstack \<Rightarrow> 'a" is
-  "\<lambda>s. more (last (Rep_tstack s))".
+fun aux :: "('var,'val,'a) stack \<Rightarrow> 'a"
+  where
+    "aux [] = undefined" |
+    "aux (h#ts) = (case more h of None \<Rightarrow> aux ts | Some v \<Rightarrow> v)"
 
 definition auxupd :: "('var,'val,'a) stack \<Rightarrow> (('var,'val,'a) stack \<Rightarrow> 'a) \<Rightarrow> ('var,'val,'a) stack" where 
-  "auxupd s f = butlast s @ [(last s)\<lparr> more := f s \<rparr>]"
-  
-lift_definition tauxupd :: "('var,'val,'a) tstack \<Rightarrow> (('var,'val,'a) tstack \<Rightarrow> 'a) \<Rightarrow> ('var,'val,'a) tstack" 
-  is "\<lambda>s f. Abs_tstack (auxupd (Rep_tstack s) (\<lambda>tstack. f (Abs_tstack tstack)))".
+  "auxupd s f \<equiv> case s of h#t \<Rightarrow> (h\<lparr> more := Some (f s)\<rparr>)#t | _ \<Rightarrow> []"
 
-lemma [intro!, simp]: "Is_tstack (Rep_tstack s)" 
-using Rep_tstack by auto
+definition captured :: "('var,'val,'a) stack \<Rightarrow> 'var \<Rightarrow> bool"
+  where "captured s v \<equiv> \<exists>frame \<in> set (butlast s). v \<in> frame_cap frame"
+
+definition base_st :: "('var,'val,'a) stack \<Rightarrow> 'var \<Rightarrow> 'val"
+  where "base_st s \<equiv> the \<circ> frame_st (last s)"
+
+definition base_aux :: "('var,'val,'a) stack \<Rightarrow> 'a"
+  where "base_aux s \<equiv> the (more (last s))"
+
+lemma [elim!]:
+  assumes "update xs x e = []"
+  obtains "xs = []"
+  using assms by (case_tac xs; auto split: if_splits)
 
 lemma Is_tstack_update: 
   assumes "Is_tstack s"
   shows "Is_tstack (update s v x)" 
-proof (induct s rule: Is_tstack_induct)
+  using assms by (induct s rule: Is_tstack_induct) (auto simp: Is_tstack_def)
+
+lemma length_update:
+  "Is_tstack s \<Longrightarrow> length (update s v x) = length s"
+  by (induct rule: Is_tstack_induct) auto
+
+lemma aux_update:
+  "Is_tstack s \<Longrightarrow> aux (update s v x) = aux s"
+  by (induct rule: Is_tstack_induct) (auto split: option.splits)
+
+lemma lookup_update:
+  "Is_tstack s \<Longrightarrow> lookup (update s v e) = (lookup s)(v := e)"
+  by (induct rule: Is_tstack_induct) (auto split: if_splits option.splits simp: fun_eq_iff)
+
+lemma captured_update:
+  "Is_tstack s \<Longrightarrow> captured (update s v e) = captured s"
+  by (induct rule: Is_tstack_induct) (auto simp: fun_eq_iff captured_def)
+
+lemma base_st_update:
+  "Is_tstack s \<Longrightarrow> base_st (update s v e) = (if captured s v then base_st s else (base_st s)(v := e))"
+  by (induct rule: Is_tstack_induct) (auto simp: base_st_def fun_eq_iff captured_def)
+
+lemma base_aux_update:
+  "Is_tstack s \<Longrightarrow> base_aux (update s v e) = base_aux s"
+  by (induct rule: Is_tstack_induct) (auto simp: base_aux_def)
+
+lemma Is_tstack_auxupd:
+  assumes "Is_tstack s"
+  shows "Is_tstack (auxupd s f)"
+  using assms by (induct s rule: Is_tstack_induct) (auto simp: Is_tstack_def auxupd_def)
+
+lemma length_auxupd:
+  "Is_tstack s \<Longrightarrow> length (auxupd s f) = length s"
+  by (induct rule: Is_tstack_induct) (auto simp: auxupd_def)
+
+lemma lookup_auxupd:
+  "Is_tstack s \<Longrightarrow> lookup (auxupd s f) = lookup s"
+  by (induct rule: Is_tstack_induct) (auto simp: auxupd_def)
+
+lemma aux_auxupd:
+  "Is_tstack s \<Longrightarrow> aux (auxupd s f) = f s"
+  by (induct rule: Is_tstack_induct) (auto simp: auxupd_def)
+
+lemma captured_auxupd:
+  "Is_tstack s \<Longrightarrow> captured (auxupd s f) = captured s"
+  by (induct rule: Is_tstack_induct) (auto simp: fun_eq_iff captured_def auxupd_def)
+
+lemma base_st_auxupd:
+  "Is_tstack s \<Longrightarrow> base_st (auxupd s f) = base_st s"
+  by (induct rule: Is_tstack_induct) (auto simp: base_st_def auxupd_def)
+
+lemma base_aux_auxupd:
+  "Is_tstack s \<Longrightarrow> base_aux (auxupd s f) = (if length s = 1 then f s else base_aux s)"
+  by (induct rule: Is_tstack_induct) (auto simp: base_aux_def auxupd_def fun_eq_iff)
+
+lemma Is_tstack_auxupd_eq:
+  "Is_tstack list \<Longrightarrow> (\<And>x. Is_tstack x \<Longrightarrow> fun1 x = fun2 x) \<Longrightarrow> auxupd list fun1 = auxupd list fun2"
+  by (induct list) (auto simp: auxupd_def)
+
+lemma base_st_lookup:
+  "Is_tstack y \<Longrightarrow> length y = 1 \<Longrightarrow> base_st y = lookup y"
+proof (induct rule: Is_tstack_induct)
   case (Base x)
-  then show ?case unfolding Is_tstack_def by simp
-qed (auto simp add: assms)
+  then show ?case by (auto simp: base_st_def fun_eq_iff split: option.splits)
+     (simp add: option.the_def)
+next
+  case (Frame x xs)
+  then show ?case by (auto simp: base_st_def fun_eq_iff split: option.splits)
+qed
 
+lemma base_aux_aux:
+  "Is_tstack y \<Longrightarrow> length y = Suc 0 \<Longrightarrow> base_aux y = aux y"
+  by (induct rule: Is_tstack_induct) (auto simp: base_aux_def fun_eq_iff split: option.splits)
+
+lift_definition tlookup :: "('var,'val,'a) tstack \<Rightarrow> 'var \<Rightarrow> 'val" is "lookup" .
+lift_definition tcaptured :: "('r,'v,'a) tstack \<Rightarrow> 'r \<Rightarrow> bool" is "captured" .
+lift_definition taux :: "('var,'val,'a) tstack \<Rightarrow> 'a" is "aux" .
+lift_definition tstack_len :: "('r,'v,'a) tstack \<Rightarrow> nat" is "length" .
+lift_definition tbase_st :: "('r,'v,'a) tstack \<Rightarrow> 'r \<Rightarrow> 'v" is "base_st" .
+lift_definition tbase_aux :: "('var,'val,'a) tstack \<Rightarrow> 'a" is "base_aux" .
+
+lift_definition tupdate :: "('var,'val,'a) tstack \<Rightarrow> 'var \<Rightarrow> 'val \<Rightarrow> ('var,'val,'a) tstack" is "update"
+  using Is_tstack_update by force
+
+lift_definition tauxupd :: "('var,'val,'a) tstack \<Rightarrow> (('var,'val,'a) tstack \<Rightarrow> 'a) \<Rightarrow> ('var,'val,'a) tstack" is "auxupd"
+  by (intro conjI Is_tstack_auxupd_eq Is_tstack_auxupd) blast+
+
+lift_definition tstack_push :: "('r,'v,'a) tstack \<Rightarrow> ('r,'v,'a option) frame_scheme \<Rightarrow> ('r,'v,'a) tstack"
+  is "\<lambda>stack frame. (\<lparr>frame_st = frame_st frame, frame_cap = frame_cap frame, \<dots> = more frame \<rparr> # stack)"
+  by (auto)
+
+abbreviation capped :: "('r,'v,'a) tstack \<Rightarrow> 'r set" where
+  "capped ts \<equiv> Collect (tcaptured ts)"
+
+definition tstack_upper :: "('r,'v,'a) tstack \<Rightarrow> ('r,'v,'a option) frame_scheme list"
+  where "tstack_upper ts = butlast (Rep_tstack ts)"
+
+text \<open>
+The number of frames within the tstack naturally tells us whether that state
+is speculative or sequential.
+\<close>
+
+abbreviation ts_is_seq where
+  "ts_is_seq ts \<equiv> tstack_len ts = 1"
+
+abbreviation ts_is_spec where
+  "ts_is_spec ts \<equiv> \<not> ts_is_seq ts"
+
+subsection \<open>@{term tupdate} Properties\<close>
+
+lemma tlength_tupdate [simp]:
+  "tstack_len (tupdate s v x) = tstack_len s"
+  by (transfer) (auto simp: length_update)
+
+lemma taux_tupdate [simp]:
+  "taux (tupdate s v x) = taux s"
+  by (transfer) (auto simp: aux_update)
+
+lemma tlookup_tupdate [simp]:
+  "tlookup (tupdate s v e) = (tlookup s)(v := e)"
+  by (transfer) (auto simp: lookup_update)
+
+lemma tcaptured_tupdate [simp]:
+  "tcaptured (tupdate x v e) = tcaptured x"
+  by (transfer) (auto simp: captured_update)
+
+lemma tbase_st_tupdate [simp]:
+  "tbase_st (tupdate s v e) = (if tcaptured s v then tbase_st s else (tbase_st s)(v := e))"
+  by (transfer) (auto simp: base_st_update)
+
+lemma tbase_aux_tupdate [simp]:
+  "tbase_aux (tupdate s v e) = tbase_aux s"
+  by (transfer) (auto simp: base_aux_update)
+
+subsection \<open>@{term tauxupd} Properties\<close>
+
+lemma tlength_tauxupd [simp]:
+  "tstack_len (tauxupd s f) = tstack_len s"
+  by (transfer) (auto simp: length_auxupd)
+
+lemma tlookup_tauxupd [simp]:
+  "tlookup (tauxupd s f) = tlookup s"
+  by (transfer) (auto simp: lookup_auxupd)
+
+lemma taux_tauxupd [simp]:
+  "taux (tauxupd s f) = f s"
+  by (transfer) (auto simp: aux_auxupd)
+
+lemma tcaptured_tauxupd [simp]:
+  "tcaptured (tauxupd x f) = tcaptured x"
+  by (transfer) (auto simp: captured_auxupd)
+
+lemma tbase_st_tauxupd [simp]:
+  "tbase_st (tauxupd s f) = tbase_st s"
+  by (transfer) (auto simp: base_st_auxupd)
+
+lemma tbase_aux_tauxupd [simp]:
+  "tbase_aux (tauxupd s f) = (if tstack_len s = 1 then f s else tbase_aux s)"
+  by (transfer) (auto simp: base_aux_auxupd)
+
+subsection \<open>@{term tstack_push} Properties\<close>
+
+lemma tlength_tpush [simp]:
+  "tstack_len (tstack_push m s) = Suc (tstack_len m)"
+  by transfer auto
+
+lemma tlookup_tpush [simp]:
+  "tlookup (tstack_push m s) = (\<lambda>x. if x \<in> frame_cap s \<and> frame_st s x \<noteq> None then the (frame_st s x) else tlookup m x)"
+  by transfer (simp add: fun_eq_iff split: option.splits)
+
+lemma taux_tpush [simp]:
+  "taux (tstack_push m s) = (case more s of Some v \<Rightarrow> v | _ \<Rightarrow> taux m)"
+  by transfer simp
+
+lemma tcaptured_tpush [simp]:
+  "tcaptured (tstack_push x s) = (\<lambda>v. v \<in> frame_cap s \<or> tcaptured x v)"
+  by (transfer)  (auto simp: captured_def fun_eq_iff)
+
+lemma tbase_st_tpush [simp]:
+  "tbase_st (tstack_push m s) = tbase_st m"
+  by transfer (auto simp: base_st_def)
+
+lemma tbase_aux_tpush [simp]:
+  "tbase_aux (tstack_push m s) = tbase_aux m"
+  by transfer (auto simp: base_aux_def)
+
+lemma tpush_eq [elim!]:
+  assumes "tstack_push mb sb = tstack_push m s"
+  obtains "mb = m" "frame_st sb = frame_st s" "frame_cap sb = frame_cap s"
+  using assms by transfer auto
+  
+subsection \<open>@{term tstack_len} Properties\<close>
+
+lemma tbase_st_tlookup [simp]:
+  "tstack_len y = 1 \<Longrightarrow> tbase_st y = tlookup y"
+  by transfer (auto simp: base_st_lookup)
+
+lemma tbase_aux_taux [simp]:
+  "tstack_len y = 1 \<Longrightarrow> tbase_aux y = taux y"
+  by transfer (auto simp: base_aux_aux)
+
+lemma [intro, simp]:
+  "tstack_len x > 0"
+  by transfer auto
+
+lemma [simp]:
+  "(tstack_len m = 0) = False"
+  by transfer auto
+
+lemma is_spec_push:
+  "ts_is_spec x \<Longrightarrow> \<exists>m s. x = tstack_push m s"
+  by transfer ((case_tac x; auto), insert surjective, blast)
+
+lemma butlast_length_eq:
+  "m \<noteq> [] \<Longrightarrow> m' \<noteq> [] \<Longrightarrow> butlast m = butlast m' \<Longrightarrow> length m = length m'"
+proof (induct m arbitrary: m')
+  case Nil
+  then show ?case by auto
+next
+  case (Cons a m)
+  then obtain b n where m: "m'=b#n" by (cases m') auto
+  hence "(a = b \<and> butlast m = butlast n \<and> n \<noteq> [] \<and> m \<noteq> []) \<or> (n = [] \<and> m = [])"
+    using Cons(4) by (auto split: if_splits)
+  thus ?case using Cons(1) by (auto simp: m)
+qed
+
+lemma tstack_upper_len_eq:
+  "tstack_upper m = tstack_upper m' \<Longrightarrow> tstack_len m = tstack_len m'"
+  unfolding tstack_upper_def by transfer (blast intro: butlast_length_eq)
+
+subsection \<open>@{term emptyFrame} Properties\<close>
+
+lemma cap_emptyFrame [simp]:
+  "frame_cap (emptyFrame w) = w"
+  by (auto simp: emptyFrame_def)
+
+lemma st_emptyFrame [simp]:
+  "frame_st (emptyFrame w) = (\<lambda>v. None)"
+  by (auto simp: emptyFrame_def)
+
+lemma more_emptyFrame [simp]:
+  "more (emptyFrame w) = None"
+  by (auto simp: emptyFrame_def)
+
+
+(*
+lemma ts_upper_of_seq [elim]: \<open>ts_is_seq m \<Longrightarrow> (tstack_upper m = [])\<close>
+unfolding  tstack_upper_def tstack_len_def 
+by (simp_all only: id_def) (simp_all add: butlast_conv_take Rep_tstackI(1) le_Suc_eq)
+
+lemma ts_is_seq_of_ts_upper [intro]: \<open>(tstack_upper m = []) \<Longrightarrow> ts_is_seq m\<close>
+unfolding  tstack_upper_def tstack_len_def 
+by (simp_all only: id_def) (simp_all add: butlast_conv_take Rep_tstackI(1) le_Suc_eq)
+*)
+
+(*
+lemma length_butlast:
+  assumes "length m = 1" "butlast m = butlast m'"
+  shows "length m' = 1 \<or> length m' = 0"
+  using assms by (cases m; cases m'; auto split: if_splits)
+
+lemma ts_is_seq_upper:
+  assumes "ts_is_seq m" "tstack_upper m = tstack_upper m'"
+  shows "ts_is_seq m'"
+  using assms using length_butlast Rep_tstack
+  unfolding  tstack_len_def tstack_upper_def Is_tstack_def
+  by auto *)
+
+
+(*
+lemma [intro!, simp]: "Is_tstack (Rep_tstack s)" 
+  using Rep_tstack by auto
+*)
+(*
 lemma Is_tstack_update2 [intro!,simp]: "Is_tstack (update (Rep_tstack fs) v x)" 
-by (simp add: Is_tstack_update)
+  by (simp add: Is_tstack_update)
+*)
 
-lemma Is_tstack_upd_len: "Is_tstack s \<Longrightarrow> length (update s v x) = length s" 
-proof (induct s)
-  case (Cons a s)
-  then show ?case
-  proof (cases "v \<in> frame_cap a")
-    case False
-    have "Is_tstack s"
-    using False Cons.prems by (rule Is_tstack_notcap)
-    then show ?thesis 
-      by (simp add: False Cons)
-  qed auto  
-qed auto
-
-lemma Is_tstack_auxupd [intro]: 
-assumes "Is_tstack s" 
-shows "Is_tstack (auxupd s f)"
-apply (induct s rule: Is_tstack_induct)
-using assms unfolding Is_tstack_def auxupd_def by auto
-  
-
-find_theorems lookup
-thm ext
-
-lemma lookup_fun_upd: 
-  assumes "Is_tstack s"
-  shows "lookup (update (s) var val) = (lookup s)(var := val)" 
-using assms
-proof (intro ext; induct s)
-  case (Cons a s)
-  then show ?case
-  proof (cases "var \<in> frame_cap a")
-    case False
-    hence "Is_tstack s" 
-      using Is_tstack_notcap Cons.prems by auto
-    thus ?thesis
-      using Cons by (cases "frame_st a x") auto
-  qed auto
-qed auto
-
-lemma lookup_update2:
-  assumes "Is_tstack s"
-  shows  "lookup (update (s) var val) var2 = (if var2 = var then val else lookup (s) var2)"
-using lookup_fun_upd assms
-by fastforce
-  
-find_theorems Abs_tstack
-  
-thm type_definition_tstack
-term more 
-
-lemma aux_update [simp]: 
-  shows "Is_tstack s \<Longrightarrow> more (last (update s v x)) = more (last s)"
-proof (induct s)
-  case (Cons a s)
-  then show ?case 
-  proof (cases "v \<in> frame_cap a")
-    case False
-    have s: "Is_tstack s"
-      using False Cons.prems by (rule Is_tstack_notcap)
-    hence "s \<noteq> []" by auto
-    moreover hence "update s v x \<noteq> []"
-      using Is_tstack_upd_len s length_0_conv by metis 
-    moreover have "more (last (update s v x)) = more (last (s))"
-      using Cons s by simp
-    ultimately show ?thesis by simp    
-  qed auto
-qed auto
-
+(*
 lemma aux_tupdate [simp]:
   shows "more (last (Rep_tstack (tupdate s v x))) = more (last (Rep_tstack s))"
+
 proof (induct s rule: tstack_induct)
   case (Base s)
   hence "Is_tstack (update [s] v x)" by (rule Is_tstack_update)
@@ -279,80 +492,14 @@ next
   hence "Is_tstack (x#xs)" by auto
   thus ?case unfolding tauxupd_def auxupd_def using Frame
   by (auto simp add: Is_tstack_ConsI Is_tstack_snoc_moreupd)
-qed
-
-lemma auxupd_Cons:
-  "xs \<noteq> [] \<Longrightarrow> auxupd (x#xs) f = x # auxupd xs (\<lambda>xs. f (x#xs))"
-unfolding auxupd_def 
-by auto
+qed *)
 
 
-
+(*
 lemma tauxupd_id [simp]: 
   "tauxupd s taux = s"
-unfolding tauxupd_def taux_def auxupd_def
-using Rep_tstackI(1)[of s]
-by (induct s) (auto simp add: Abs_tstack_inverse)
-
-lemma taux_tupd [simp]: 
-  "taux (tupdate s v x) = taux s" 
-unfolding taux_def tupdate_def
-proof (induct s rule: tstack_induct)
-  case (Base x)
-  then show ?case
-    using RepAbs_id[OF Base] RepAbs_id[OF Is_tstack_update[OF Base]] aux_update 
-    by auto
-next
-  case (Frame x xs)
-  then show ?case
-  using aux_update by fastforce
-qed  
-
-lemma tlookup_tauxupd [simp]:
-  "tlookup (tauxupd s f) v = tlookup s v" 
-unfolding tlookup_def tauxupd_def
-proof (induct s arbitrary: f v rule: tstack_induct)
-  case (Base x)
-  then show ?case unfolding auxupd_def by (simp add: Is_tstack_def)
-next
-  case (Frame x xs)
-  hence "xs \<noteq> []" by auto
-  with Frame have 1: "Is_tstack (x#xs)" by auto
-  with Frame have 2: "Is_tstack (auxupd (xs) (\<lambda>x. f (Abs_tstack x)))" by auto
-  with 1 have 3: "Is_tstack (auxupd (x # xs) (\<lambda>x. f (Abs_tstack x)))" by auto
-  note Is_tstack = \<open>Is_tstack xs\<close> 1 2 3 
-  
-  have "lookup (auxupd xs (\<lambda>xx. f (Abs_tstack (x#RepAbs_tstack xx)))) v = lookup xs v"
-    using Is_tstack Frame(1)[of "\<lambda>y. f (Abs_tstack (x#(Rep_tstack y)))"]
-    by (simp add: Is_tstack_auxupd)
-  hence "lookup ( (auxupd xs (\<lambda>xx. f (Abs_tstack (x#xx))))) v = lookup ( xs) v"
-    by (simp add: Is_tstack(1) auxupd_def)
-
-  hence "lookup (x # auxupd xs (\<lambda>y. f (Abs_tstack (x#y)))) v = lookup (x # xs) v" 
-    by (cases "frame_st x v") auto
-  hence "lookup (auxupd (x # xs) (\<lambda>x. f (Abs_tstack x))) v = lookup (x # xs) v"
-    using \<open>xs \<noteq> []\<close> auxupd_Cons by (simp add: auxupd_def)
-  then show ?case using Is_tstack by simp
-qed
-
-
-lift_definition tstack_push :: "('r,'v,'a) tstack \<Rightarrow> ('r,'v) frame \<Rightarrow> ('r,'v,'a) tstack"
-is
-  "\<lambda>stack frame. Abs_tstack (\<lparr>frame_st = frame_st frame, frame_cap = frame_cap frame, \<dots> = undefined \<rparr> # Rep_tstack stack)"
-  .
-
-lift_definition tstack_top :: "('r,'v,'a) tstack \<Rightarrow> ('r,'v,'a) frame_scheme"
-is
-  "\<lambda>stack. hd (Rep_tstack stack)".
-
-definition tstack_base_st :: "('r,'v,'a) tstack \<Rightarrow> 'r \<Rightarrow> 'v" where
-"tstack_base_st ts = the \<circ> frame_st (last (Rep_tstack ts))"
-
-definition tstack_len :: "('r,'v,'a) tstack \<Rightarrow> nat" where
-"tstack_len ts = length (Rep_tstack ts)"
-
-lift_definition tstack_upper :: "('r,'v,'a) tstack \<Rightarrow> ('r,'v,'a) frame_scheme list" is
-"\<lambda>ts. butlast (Rep_tstack ts)".
+  by transfer (auto simp: auxupd_def split: list.splits)
+*)
 
 (*
 interpretation stack: state
@@ -403,16 +550,6 @@ next
   then show ?case by simp
 qed 
 *)
-
-lemma tupdate_len:
-  "tstack_len t = tstack_len (tupdate t x a)"
-  by (simp add: Is_tstack_upd_len tstack_len_def tupdate.rep_eq)
-
-lemma tauxupd_len:
-  "tstack_len t = tstack_len (tauxupd t f)"
-  unfolding tstack_len_def tauxupd_def
-  by (induct t) (auto simp add: Is_tstack_def auxupd_def)
-
 
 end
 
